dummy support for call

examples/sgx/Ast.fst
@@ -9,12 +9,12 @@ let u64 = UInt64.t
 
 type exp =
  |Register of string
- |Constant of nat
+ |Constant of u64
 
 type stmt = 
- |Store of nat*exp * exp
+ |Store of u64*exp * exp
  |Assign of exp * exp
- |Load of exp * nat* exp
+ |Load of exp * u64* exp
  |Seq of (list stmt)
  |If of exp * (list stmt) * (list stmt)
  |Jump of exp
