examples/sgx/Interpreter.fst
@@ -5,6 +5,7 @@ open SGXState
 open FStar.Array
 open FStar.UInt64
 open FStar.List
+open Util
 open Ast
 
 exception Halt
@@ -14,6 +15,7 @@ let u64 = UInt64.t
 val defensive: (array u64) -> (array u64) ->nat-> nat-> sgxstate
 let defensive regs buf base size = 
   let read' (regname:string) = 
+       (* What should regs structure be? *)
        0uL
     in
   let write' (regname:string) (value:u64) = 
@@ -27,24 +29,42 @@ let defensive regs buf base size =
     in
    Mksgxstate read' write' load' store'
 	
+(* Should look into the call table from manifest and fetch the corresponding function
+ *)
+let decode insaddr = [Skip]
 
+let get_register_name = function
+ | Register r -> r
+ | _ -> raise Halt
 
 val eval: sgxstate -> exp -> u64
 let eval (env:sgxstate) = function
  | Register r -> env.read r 
- | Constant n -> 0uL
+ | Constant n -> n
 
-let step (env:sgxstate) = function 
+val step : sgxstate -> stmt -> unit
+val steps : sgxstate -> (list stmt) -> unit
+
+let rec step (env:sgxstate) = function 
   | Skip -> ()
   | Store(n, ea, ev)-> 
        let a = eval env ea in
        let v = eval env ev in 
-       env.store n v 0
+       env.store (cast_to_nat n) v (cast_to_nat a)
+  | Load (reg, n, ea) ->
+       let a = eval env ea in
+       let value = env.load (cast_to_nat n) (cast_to_nat a) in
+       let regname = get_register_name reg in
+       env.write regname value
+  | Call e ->
+       let fentry = eval env e in
+	(* Convert this to sequence of instructions *)
+	steps env (decode fentry)
 
-let steps (env:sgxstate) instr = List.iter (fun elem->step env elem ) instr  
+and steps (env:sgxstate) instr = List.iter (fun elem->step env elem ) instr  
 
 val ustar:(array u64)->(array u64) -> nat ->unit->unit
 let ustar regs buf base entry = 
   let size = 1000 in
   let mem = defensive regs buf base size in
-  steps mem [(Store(1,(Register "rax"),(Register "rcx")))] 
+  steps mem [(Store(1uL,(Register "rax"),(Register "rcx")))] 
